proof simplification 3.3

strandlib.v
@@ -1,9 +1,10 @@
 Require Import Logic List ListSet Arith Peano_dec Omega Ensembles.
 Require Import Coq.Sets.Constructive_sets.
 Require Import Finite_sets_facts Finite_sets Relation_Definitions.
-Require Import Relation_Operators.
+Require Import Relation_Operators Operators_Properties.
 Require Import strictorder set_rep_equiv util.
 Require Import finite_set_builder.
+Require Import CoLoRRelDec CoLoRRelSub.
 Require Import LibTactics.
 
 Require Import strandspace.
@@ -13,17 +14,808 @@ Import ListNotations.
 Open Scope ss_scope.
 
 Hint Resolve Coq.Sets.Constructive_sets.Add_not_Empty Noone_in_empty.
-Hint Unfold Origin.
+
+
+
+Definition eq_msg_dec : forall x y : Msg,  
+  {x = y} + {x <> y}.
+Proof.
+  decide equality.
+Qed.
+Hint Resolve eq_msg_dec.
+
+Definition eq_smsg_dec : forall x y : SMsg,  
+  {x = y} + {x <> y}.
+Proof.
+ intros. decide equality.
+Qed. 
+Hint Resolve eq_smsg_dec.
+
+Definition eq_strand_dec : forall x y : Strand,  
+  {x = y} + {x <> y}.
+Proof.
+ intros. decide equality.
+Qed.
+Hint Resolve eq_strand_dec.
+
+
+Lemma node_smsg_msg_tx : forall n t,
+smsg(n) = (+ t) ->
+msg(n) = t.
+Proof.
+  intros n t nsmsg.
+  unfold msg. rewrite nsmsg. reflexivity. 
+Qed.
+Hint Resolve node_smsg_msg_tx.
+
+Lemma node_smsg_msg_rx : forall n t,
+smsg(n) = (- t) ->
+msg(n) = t.
+Proof.
+  intros n t nsmsg.
+  unfold msg. rewrite nsmsg. reflexivity. 
+Qed.
+Hint Resolve node_smsg_msg_rx.
+
+Definition eq_node_dec : forall x y : Node,
+ {x = y} + {x <> y}.
+Proof.
+  intros [[xs xn] xp] [[ys yn] yp].
+  destruct (eq_strand_dec xs ys) as [EQs | NEQs]; subst.
+  destruct (eq_nat_dec xn yn) as [EQn | NEQn]; subst.
+  left. rewrite (proof_irrelevance (lt yn (length ys)) xp yp). reflexivity.
+
+  right. intros C. inversion C. auto.
+  right. intros C. inversion C. auto.
+Qed.
+Hint Resolve eq_node_dec.
+
+Lemma eq_nodes : forall x y : Node,
+index(x) = index(y) ->
+strand(x) = strand(y) ->
+x = y.
+Proof.
+  intros [[xs xn] xp] [[ys yn] yp] eq_index eq_strand.
+  simpl in eq_index. simpl in eq_strand. subst.
+  rewrite (proof_irrelevance (lt yn (length ys)) xp yp). reflexivity.
+Qed.
+Hint Resolve eq_nodes.
+
+
+Lemma nodes_eq : forall x y : Node,
+x = y ->
+index(x) = index(y) /\
+strand(x) = strand(y).
+Proof.
+  intros x y xyeq.
+  subst. auto.
+Qed.
+Hint Resolve nodes_eq.
+
+Lemma node_imp_strand_nonempty : forall s n,
+strand(n) = s ->
+length s > 0.
+Proof.
+  intros s n Hns.
+  destruct n. destruct x.
+  destruct n. simpl in l.
+  destruct s.
+  Case "s = []".
+    assert (s0 = nil). auto.
+  subst. inversion l.
+  Case "s = s :: s1".
+    simpl. omega.
+    simpl in l. 
+    assert (s0 = s). auto.
+    rewrite <- H.
+    omega.
+Qed.
+Hint Resolve node_imp_strand_nonempty.
+
+
+Lemma index_len_node : forall n,
+(index n) < length (strand n).
+Proof.
+  intros n.
+  destruct n. simpl. omega.
+Qed.
+Hint Resolve index_len_node.
+
+Lemma node_indexing_equiv : forall n,
+nth_error (strand n) (index n) = Some (smsg n).
+Proof.
+  intros n.
+  unfold smsg. destruct node_smsg_valid. 
+  destruct n. simpl in *.
+  destruct x0.
+  rewrite e. simpl. reflexivity.
+Qed.
+Hint Resolve node_indexing_equiv.
+
+Lemma strand_node : forall (s: Strand) (i: nat),
+i < length s ->
+exists n, strand n = s /\ index n = i.
+Proof.
+  intros s i len.  
+  eexists (exist _ (s,i) _). simpl.
+  split; reflexivity.
+Grab Existential Variables.
+  simpl. exact len.
+Qed.
+Hint Resolve strand_node.
+
+Lemma comm_dec : forall x y,
+{x --> y} + {~ x --> y}.
+Proof.
+  intros x y.
+  remember (smsg x) as xsmsg. remember (smsg y) as ysmsg.
+  remember (strand x) as xstrand. remember (strand y) as ystrand.
+  destruct xsmsg.
+  Case "x (tx m)".
+    destruct ysmsg.
+    SCase "y (tx m0)".
+      right. intros contracomm. inversion contracomm; subst.
+      destruct H as [[xtx yrx] strandneq].
+      rewrite <- Heqysmsg in yrx. inversion yrx.      
+    SCase "y (rx m0)".
+      destruct (eq_msg_dec m m0) as [msgeq | msgneq].
+      SSCase "m = m0".
+        destruct (eq_strand_dec xstrand ystrand) as [strandeq | strandneq].
+        SSSCase "strands eq".
+          right. intros contracomm.
+          inversion contracomm; subst. destruct H as [msgs strandsneq].
+          apply strandsneq. exact strandeq. 
+        SSSCase "strands neq".
+          subst m0. left.
+          apply (comm x y m). split. split.
+          auto. auto. subst. exact strandneq.        
+      SSCase "m <> m0".
+        right. intros contracomm. inversion contracomm; subst. 
+        destruct H as [[xtx yrx] strandneq].
+        apply msgneq. rewrite <- Heqxsmsg in xtx.
+        rewrite <- Heqysmsg in yrx. inversion xtx; subst. 
+        inversion yrx; subst. reflexivity.
+  Case "x (rx m)".
+    right.
+    intros contracomm. inversion contracomm; subst.
+    destruct H as [[xtx yrx] strandneq].
+    rewrite <- Heqxsmsg in xtx. inversion xtx.
+Qed.
+Hint Resolve comm_dec.
+
+
+Theorem comm_irreflexivity : forall n,
+~ n --> n.
+Proof.
+  intros n contraedge.
+  inversion contraedge; subst.
+  destruct H as [[txsmsg rxsmsg] strandneq].
+  apply strandneq. reflexivity.
+Qed.
+Hint Resolve comm_irreflexivity.
+
+Theorem comm_antisymmetry : 
+Antisymmetric Node Comm.
+Proof.
+  intros n m Hcomm contra.
+  assert False.
+  inversion Hcomm; subst.
+  inversion contra; subst.
+  destruct H as [H Hneq_s].
+  destruct H as [Htx1 Hrx1].
+  destruct H0 as [H Hneq_s2].
+  destruct H as [Htx2 Hrx2].
+  rewrite Htx2 in Hrx1. inversion Hrx1.
+  inversion H.
+Qed.
+Hint Resolve comm_antisymmetry.
+
+Lemma succ_dec : forall x y,
+{x ==> y} + {~ x ==> y}.
+Proof.
+  intros x y.
+  remember (index x) as xi. remember (index y) as yi.
+  remember (strand x) as xstrand. remember (strand y) as ystrand.
+  destruct (eq_strand_dec xstrand ystrand) as [seq | sneq].
+  Case "strands eq".
+    destruct (eq_nat_dec yi (S xi)) as [succi | wrongi].
+    SCase "yi = S xi". left. apply (succ x y). rewrite <- Heqxstrand.
+      rewrite <- Heqystrand.  exact seq. omega.
+    SCase "yi <> S xi".
+      right. intros contrasucc. apply wrongi. inversion contrasucc; subst; omega.
+  Case "strands neq".
+    right. intros contrasucc. apply sneq. inversion contrasucc; subst; auto.
+Qed.  
+Hint Resolve succ_dec.
+
+
+Theorem succ_irreflexivity : forall n,
+~n ==> n.
+Proof.
+  intros n edge.
+  inversion edge; subst. omega.
+Qed.
+Hint Resolve succ_irreflexivity.
+
+Theorem succ_antisymmetry :
+Antisymmetric Node Successor.
+Proof.
+  intros n m Hpe1 Hpe2.
+  destruct Hpe1. destruct Hpe2.
+  rewrite <- H0 in H2. omega.
+Qed.
+Hint Resolve succ_antisymmetry.
+
+Lemma single_succ : forall x y z,
+x ==> y ->
+x ==> z ->
+y = z.
+Proof.
+  intros x y z xy xz.
+  destruct xy.
+  destruct xz.
+  apply eq_nodes; auto; try omega; try congruence.
+Qed.
+Hint Resolve single_succ.
+
+Lemma spath_imp_eq_strand : forall x y,
+x ==>+ y -> strand(x) = strand(y).
+Proof.
+  intros x y path.
+  induction path.
+  Case "step".
+    destruct H; auto.
+  Case "trans".
+    rewrite IHpath1.
+    rewrite IHpath2.
+    reflexivity.
+Qed.
+Hint Resolve spath_imp_eq_strand.
+
+Lemma spath_imp_index_lt : forall x y,
+x ==>+ y -> index(x) < index(y).
+Proof.
+  intros x y path.
+  induction path.
+  Case "step". inversion H; subst. omega.
+  Case "trans". omega.
+Qed.
+Hint Resolve spath_imp_index_lt.
+
+Lemma path_step_holds : forall x x' y,
+x ==>+ y ->
+x ==> x' ->
+x' = y \/ x' ==>+ y.
+Proof.
+  intros x x' y path. generalize dependent x'.
+  apply clos_trans_t1n in path.
+  induction path.
+    intros. left. eapply single_succ; eauto.
+    intros.
+    forwards*: (single_succ x y x'). subst.
+    right. apply clos_t1n_trans in path. auto.
+Qed.
+Hint Resolve path_step_holds.
+
+Lemma spath_from_props : forall x y,
+index(x) < index(y) ->
+(strand x) = (strand y) ->
+x ==>+ y.
+Proof.
+  intros x.
+  destruct x as [[xs xi] xp]. simpl in *. 
+  induction xi.
+    intros y ind streq.
+    destruct y as [[ys yi] yp]. simpl in *. 
+    induction yi. omega. 
+      destruct yi.
+        constructor. constructor. auto. simpl. reflexivity.
+        assert (snd (ys, S yi) < length (fst (ys, S yi))) as yp'. simpl. omega.
+        apply (t_trans Node Successor
+                 (exist (fun n : Strand * nat => snd n < length (fst n)) (xs, 0) xp)
+                 (exist (fun n : Strand * nat => snd n < length (fst n)) (ys, S yi) yp')
+                 (exist (fun n : Strand * nat => snd n < length (fst n)) (ys, S (S yi)) yp)).
+        apply IHyi. omega.
+        constructor. constructor. auto. simpl. omega.
+    intros y ind streq.
+    assert (snd (xs, xi) < length (fst (xs, xi))) as xp'. simpl. omega.
+    assert (exist (fun n : Strand * nat => snd n < length (fst n)) (xs, xi) xp') ==>
+         (exist (fun n : Strand * nat => snd n < length (fst n)) (xs, S xi) xp).
+      constructor. constructor. auto. simpl. omega.
+    assert (xi < index y). omega.
+    remember (IHxi xp' y H0 streq).
+    destruct (path_step_holds 
+              (exist (fun n : Strand * nat => snd n < length (fst n)) (xs, xi) xp')
+              (exist (fun n : Strand * nat => snd n < length (fst n)) (xs, S xi) xp)
+              y
+              s
+              H).
+    apply nodes_eq in H1. destruct H1. simpl in *.
+    constructor. constructor; auto. omega.
+    assumption.
+Qed.
+Hint Resolve spath_from_props.
+
+Lemma spath_irreflexivity : forall n,
+~ n ==>+ n.
+Proof.
+  intros n contra.
+  apply spath_imp_index_lt in contra.
+  omega.
+Qed.
+Hint Resolve spath_irreflexivity.
+
+Theorem spath_transitivity :
+Transitive Node StrandPath.
+Proof.
+  intros i j k Hij Hjk.
+  apply (t_trans Node Successor i j k Hij Hjk).
+Qed.
+Hint Resolve spath_transitivity.
+
+Lemma ssedge_dec : forall x y,
+{x =-> y} + {~x =-> y}.
+Proof.
+  intros x y.
+  destruct (comm_dec x y) as [cxy | nocxy].
+  Case "Comm x y".
+    left. left. exact cxy.
+  Case "~Comm x y".
+    destruct (succ_dec x y) as [pxy | nopxy].
+    SCase "Successor x y".
+      left. right. exact pxy.
+    SCase "~Successor x y".
+      right. intros contrass.
+       destruct contrass.
+       SSCase "false Comm".
+         apply nocxy; exact H.
+       SSCase "false Successor".
+         apply nopxy; exact H.
+Qed.
+Hint Resolve ssedge_dec.
+
+Theorem ssedge_irreflexivity : forall n,
+~ n =-> n.
+Proof.
+  intros n Hedge.
+  inversion Hedge; subst; auto.
+  eapply (comm_irreflexivity); eauto.
+  eapply (succ_irreflexivity); eauto.
+Qed.
+Hint Resolve ssedge_irreflexivity.
+
+Theorem ssedge_antisymmetry :
+Antisymmetric Node SSEdge.
+Proof.
+  intros n m Hss Hcontra.
+  inversion Hss; subst. inversion Hcontra; subst.
+  apply (comm_antisymmetry n m H) in H0. exact H0.
+  assert False.
+  inversion H; subst. inversion H0; subst.
+  inversion H1. apply H5. symmetry. exact H2.
+  inversion H1.
+  assert False.
+  inversion Hcontra; subst. inversion H; subst.
+  inversion H0; subst. inversion H3. apply H5.
+  symmetry. exact H1.
+  inversion H; subst. inversion H0; subst.
+  omega. inversion H0.
+Qed.
+Hint Resolve ssedge_antisymmetry.
+
+Theorem spath_imp_sspath : forall i j,
+i ==>+ j -> i << j.
+Proof.
+  unfold SSPath.
+  intros i j Hpath.
+  induction Hpath.
+  constructor. right. exact H.
+  apply (t_trans Node SSEdge x y z IHHpath1 IHHpath2).
+Qed.  
+Hint Resolve spath_imp_sspath.
+
+Theorem sspath_transitivity :
+Transitive Node SSPath.
+Proof.
+  unfold SSPath.
+  intros i j k Hij Hjk.
+  apply (t_trans Node SSEdge i j k Hij Hjk).
+Qed.
+Hint Resolve sspath_transitivity.
+
+Theorem sspatheq_opts: forall n m,
+n <<* m -> n << m \/ n = m.
+Proof.
+  intros n m Hpatheq.
+  induction Hpatheq.
+  left. apply t_step. exact H.
+  right. reflexivity.
+  destruct IHHpatheq1 as [pathxy | eqxy].
+    destruct IHHpatheq2 as [pathyz | eqyz].
+      left. eapply t_trans. exact pathxy. exact pathyz.
+      subst y. left. exact pathxy.
+    destruct IHHpatheq2 as [pathyz | eqyz].
+      subst x. left. exact pathyz.
+      right. subst. reflexivity.
+Qed.
+Hint Resolve sspatheq_opts.
+
+Theorem sspatheq_transitivity :
+Transitive Node SSPathEq.
+Proof.
+  unfold Transitive.
+  intros i j k Hij Hjk.
+  destruct Hij. 
+    eapply rt_trans. eapply rt_step. exact H. 
+    exact Hjk. exact Hjk. 
+    eapply rt_trans. exact Hij1. eapply rt_trans.
+    exact Hij2. exact Hjk.
+Qed.
+
+
+Lemma bundle_ssedge_inclusion : forall (B: Bundle) (n m: Node),
+n =-> m ->
+(In Node (Nodes B) n <-> In Node (Nodes B) m).
+Proof.
+  intros B n m ssedge. split; intros Hin.
+  destruct B as [N E finN finE valE uniqtx acyc]; simpl in *.
+  apply valE in ssedge. apply valE. constructor 2.
+  exists n. exact ssedge.
+  destruct B as [N E finN finE valE uniqtx acyc].
+  apply valE in ssedge. apply valE. constructor 1.
+  exists m. exact ssedge.
+Qed.
+Hint Resolve bundle_ssedge_inclusion.
+
+Lemma sspath_imp_ssedge_l : forall x y,
+x << y ->
+exists x', x =-> x'.
+Proof.
+  intros x y sspath.
+  induction sspath.
+  exists y. exact H.
+  exact IHsspath1.
+Qed.  
+Hint Resolve sspath_imp_ssedge_l.
+
+Lemma sspath_imp_ssedge_r : forall x y,
+x << y ->
+exists y', y' =->  y.
+Proof.
+  intros x y sspath.
+  induction sspath.
+  exists x. exact H.
+  exact IHsspath2.
+Qed.  
+Hint Resolve sspath_imp_ssedge_r.
+
+Lemma restricted_to_set : forall (B:Bundle),
+exists s, is_restricted SSEdge s /\
+forall x, ListSet.set_In x s <-> In Node (Nodes B) x.
+Proof.
+  intros B.
+  destruct B as [N E finN finE valE uniqtx acyc]; simpl in *.
+  destruct valE as [EimpInN EimpSSEdge].
+  destruct (ensemble_imp_set Node eq_node_dec N finN) 
+    as [s [inAll [nodup [n [slen scard]]]]].
+  exists s.
+  split.
+  intros x y sspath.
+  split.
+  apply inAll. apply EimpInN. constructor. exists y. 
+  apply EimpSSEdge. exact sspath.
+  apply inAll. apply EimpInN. constructor 2. exists x. 
+  apply EimpSSEdge. exact sspath.
+  exact inAll.
+Qed.
+
+Lemma sspath_dec : forall (B: Bundle) (s: ListSet.set Node),
+node_set_Ensemble_equiv s (Nodes B) ->
+is_restricted SSEdge s ->
+forall x y, {x << y} + {~x << y}.
+Proof.
+  intros B s bset restrict.
+  destruct B as [N E finN finE valE uniqtx acyc]; simpl in *.
+  intros x y.
+  remember (restricted_dec_clos_trans_dec 
+              eq_node_dec 
+              ssedge_dec 
+              restrict) as alldec.
+  apply alldec.
+Qed.
+Hint Resolve sspath_dec.
+
+Lemma neq_sspatheq_imp_sspath : forall (x y: Node),
+x <> y ->
+x <<* y ->
+x << y.
+Proof.
+  intros x y neq patheqxy.
+  induction patheqxy.
+  Case "SSEdge x y".
+    apply t_step. exact H.
+  Case "x = y". assert False as F. apply neq. reflexivity. inversion F.
+  Case "x y z".
+    destruct (eq_node_dec y z) as [eqyz | neqyz].
+    SCase "y = z". subst y. apply IHpatheqxy1. exact neq.
+    SCase "y <> z". 
+      destruct (eq_node_dec x y) as [eqxy | neqxy].
+      SSCase "x = y". subst x. apply IHpatheqxy2. exact neqyz.
+      SSCase "x <> y". eapply t_trans. apply IHpatheqxy1. exact neqxy.
+        apply IHpatheqxy2. exact neqyz.
+Qed.      
+Hint Resolve neq_sspatheq_imp_sspath.
+
+Lemma sspatheq_trans_cycle : forall (x y: Node),
+x <> y ->
+x <<* y ->
+y <<* x ->
+x << x.
+Proof.
+  intros x y neq patheqxy patheqyx.
+  eapply t_trans.
+  Case "path x y".
+    eapply neq_sspatheq_imp_sspath. exact neq. exact patheqxy.
+  Case "path y x".
+    eapply neq_sspatheq_imp_sspath. intros contra. subst.
+    apply neq. reflexivity.
+    exact patheqyx.
+Qed.
+Hint Resolve sspatheq_trans_cycle.
+
+Lemma Origin_imp_strict_defs : forall I t n,
+(forall t', t <st t' <-> In Msg I t') ->
+Origin t n ->
+Origin_with_Ex_Set t n.
+Proof.
+  intros I t n Iprop Orig.
+  exists I. split. exact Iprop.
+  destruct Orig as [ntx [nsub nosucc]].
+  split. exists (msg n).
+  split. apply Iprop in nsub. exact nsub.
+  destruct ntx. erewrite node_smsg_msg_tx. exact H. exact H.
+  intros n' succ contraIn.
+  apply nosucc in succ. apply Iprop in contraIn. contradiction.
+Qed.
+Hint Resolve Origin_imp_strict_defs.
+
+(* Lemma 2.7a (partial order)  *)
+Lemma bundle_partial_order : forall (B:Bundle),
+Order Node SSPathEq.
+Proof.
+  intros B.
+  split.
+  Case "Reflexivity".
+    intros x. apply rt_refl. 
+  Case "Transitivity".
+    intros x y z xy yz.
+    eapply rt_trans. exact xy. exact yz.
+  Case "AntiSymmetry".
+    intros x y xy yz.
+    destruct B as [N E finN finE valE uniqtx acyc]; simpl in *.
+    destruct (eq_node_dec x y) as [xyeq | xyneq].
+    SCase "x = y". exact xyeq.
+    SCase "x <> y". 
+      assert (x << x) as contraxx.
+        eapply sspatheq_trans_cycle. exact xyneq.
+        exact xy. exact yz. apply acyc in contraxx. inversion contraxx.
+Qed.
+Hint Resolve bundle_partial_order.
+
+Lemma sspath_strict_order : forall (B: Bundle),
+StrictOrder Node SSPath.
+Proof.
+  intros B.
+  destruct B as [N E finN finE valE uniqtx acyc]; simpl in *.
+  split.
+  Case "Irreflexivity".
+    intros x. apply acyc.
+  Case "Transitivity".
+    apply sspath_transitivity.
+Qed.
+Hint Resolve sspath_strict_order.
+
+(* Lemma 2.7b (non-empty subsets contain minimal members) *)
+Lemma bundle_subset_minimal : forall B N',
+Included Node N' (Nodes B) ->
+N' <> Empty_set Node ->
+exists min, set_minimal N' min.
+Proof.
+  intros B N' incl nempty.
+  remember B as bundle.
+  destruct bundle as [N E finN finE valE uniqtx acyc]; simpl in *.
+  assert (Finite Node N') as finN'. eapply Finite_downward_closed.
+    exact finN. exact incl.
+  destruct (finite_cardinal Node N' finN') as [n card].
+  destruct n. inversion card. rewrite H in nempty.
+  assert False as F. apply nempty. reflexivity. inversion F.
+  destruct (restricted_to_set B) as [s [restricted setequiv]].
+  assert (forall x y, {x << y} + {~ x << y}) as rdec.
+  apply (sspath_dec B s). exact setequiv. exact restricted.  
+  destruct (minimal_finite_ensemble_mem 
+              Node 
+              eq_node_dec 
+              SSPath 
+              rdec
+              (sspath_strict_order B) 
+              N' 
+              n 
+              card) as [min [minIn nolt]].
+  exists min. split. exact minIn. exact nolt.
+Qed.
+Hint Resolve bundle_subset_minimal.
+
+(* Lemma 2.8 - set minimal is tx *)
+Lemma minimal_is_tx : forall B N',
+Included Node N' (Nodes B) ->
+(forall m m' : Node, (In Node (Nodes B) m 
+               /\ In Node (Nodes B) m'
+               /\ msg(m) = msg(m')) -> (* ADDED in N conditions *)
+               (In Node N' m <-> In Node N' m')) ->
+forall n, set_minimal N' n ->
+is_tx n.
+Proof.
+  intros B N' sub incl n setmin.
+  remember B as bundle.
+  destruct bundle as [N E finN finE valE uniqtx acyc]; simpl in *.
+  assert ((Nodes B) = N) as NB. subst B. simpl. reflexivity.
+  remember (smsg n) as nsmsg. symmetry in Heqnsmsg.
+  destruct nsmsg.
+  exists m. exact Heqnsmsg.
+  unfold ExistsUniqueTx in uniqtx.
+  assert (In Node N n) as nIn. destruct setmin; auto.
+  destruct (uniqtx n m nIn Heqnsmsg) as [[ntx [ntxsmsg [commn inE]]] uniq].
+  assert False as F. destruct setmin. apply (H0 ntx). eapply incl.
+    split. rewrite <- NB. eapply bundle_ssedge_inclusion. 
+    constructor. exact commn. rewrite NB. exact nIn. 
+    split. exact nIn. apply node_smsg_msg_tx in ntxsmsg. 
+    apply node_smsg_msg_rx in Heqnsmsg. rewrite Heqnsmsg. exact ntxsmsg. 
+    exact H. constructor. constructor. exact commn.
+  inversion F.
+Qed.
+Hint Resolve minimal_is_tx.
+
+(* Lemma 2.9 originating occurrence at minimal element *)
+Lemma min_origin : forall B N' n t,
+(forall m, (In Node (Nodes B) m 
+           /\ Subterm t (msg(m))) -> 
+           In Node N' m) ->
+(forall m, In Node N' m -> 
+           (In Node (Nodes B) m 
+           /\ Subterm t (msg(m)))) ->
+set_minimal N' n ->
+Origin t n.
+Proof.
+  intros B N' n t N'deff N'defb nmin.
+  remember B as bundle.
+  destruct bundle as [N E finN finE valE uniqtx acyc]; simpl in *.
+  assert (N = Nodes B) as NB. subst B. simpl; reflexivity.
+  assert (In Node N' n) as nIn. destruct nmin; auto.
+  assert (t <st (msg n)) as tsubn.
+    apply (N'defb n) in nIn. destruct nIn; auto.
+  assert (is_tx n) as nistx.
+    assert (Included Node N' N) as incl.
+      intros x xIn. apply N'defb in xIn. destruct xIn; auto.
+    rewrite NB in incl. apply (minimal_is_tx B N' incl).
+    intros x y eqmsg.
+    destruct eqmsg as [xIn [yIn eqmsg]].
+    split; intros Hin.
+    Case "m in -> m' in".
+      apply N'defb in Hin. destruct Hin as [xInN tsubx]. 
+      assert (Subterm t (msg y)) as ysubt. rewrite <- eqmsg.
+        exact tsubx.
+      apply N'deff. split. rewrite NB. exact yIn. exact ysubt.
+    Case "m' in -> m in".
+      apply N'defb in Hin. destruct Hin as [yInN tsuby].
+      apply N'deff. split. rewrite NB. exact xIn. 
+      assert (Subterm t (msg x)) as xsubt. rewrite eqmsg.
+        exact tsuby.
+      exact xsubt. 
+    exact nmin.
+  split. exact nistx.
+  split. exact tsubn.
+  intros n' succn' contrasub.
+  assert (In Node N' n') as n'In.
+    apply N'deff. split.
+    destruct valE as [pairImpN HInEedge].
+    apply pairImpN. left.
+    destruct (sspath_imp_ssedge_l n' n succn') as [x n'edge].
+    exists x. apply HInEedge. exact n'edge. exact contrasub.
+  destruct nmin as [nIn2 noprev]. apply (noprev n'). exact n'In.
+  exact succn'.
+Qed.
+Hint Resolve min_origin.
+
+(* Proposition 2.12 *)
+Lemma encr_subterm_imp : forall k k' h h',
+k <> k' ->
+{h'}^[k'] <st {h}^[k] ->
+{h'}^[k'] <st h.
+Proof.
+  intros k k' h h' kneq st.
+  inversion st; subst.
+  assert False. apply kneq. reflexivity. contradiction.
+  exact H1.
+Qed.
+Hint Resolve encr_subterm_imp.
+
+Lemma st_dec : forall a b,
+{a <st b} + {~ a <st b}.
+Proof.
+  intros a b.
+  induction b.
+  Case "b = txt".
+    destruct a.
+    SCase "a = txt".
+      destruct (eq_text_dec t t0).
+        subst t. left. auto.
+        right. intros contra. inversion contra. 
+        symmetry in H1. contradiction.
+    SCase "a = key". right. intros contra. inversion contra.
+    SCase "a = join". right. intros contra. inversion contra.
+    SCase "a = encr". right. intros contra. inversion contra.
+  Case "b = key".
+    destruct a.
+    SCase "a = txt". right. intros contra. inversion contra.
+    SCase "a = key".
+      destruct (eq_key_dec k k0).
+        subst k. left. auto.
+        right. intros contra. inversion contra. 
+        symmetry in H1. contradiction.
+    SCase "a = join". right. intros contra. inversion contra.
+    SCase "a = encr". right. intros contra. inversion contra.
+  Case "b = join".
+    destruct IHb1.
+    SCase "a <st b1". left. apply st_join_l. exact s.
+    SCase "~a <st b1". 
+      destruct IHb2.
+      SSCase "a <st b2". left. apply st_join_r. exact s.
+      SSCase "~a <st b2". 
+        destruct (eq_msg_dec a (b1 * b2)).
+        SSSCase "a = b1 * b2".
+          subst a. left. constructor.
+        SSSCase "a <> b1 * b2".
+          right. intros contra. inversion contra; subst; try(contradiction).
+          apply n1. reflexivity.
+  Case "b = encr".
+    destruct IHb.
+      left. apply st_encr. exact s.
+      destruct (eq_msg_dec a ({b}^[k])). subst.
+      left. constructor.
+      right. intros contra. inversion contra. subst.
+      apply n0. reflexivity.
+      contradiction.
+Qed.
+Hint Resolve st_dec.
+
+Fixpoint st_on_strand (t:Msg) (s:Strand) : bool :=
+match s with
+| nil => false
+| x :: xs => 
+  if st_dec t (smsg_msg x)
+  then true
+  else st_on_strand t xs
+end.
+
+
+Theorem align_dec : forall s,
+{RegularStrand s} + {PenetratorStrand s}.
+Proof.
+  intros s. destruct (set_In_dec eq_strand_dec s Protocol); auto.
+Qed.
+Hint Resolve align_dec.
 
 Lemma origin_tx : forall n t,
 Origin t n ->
 is_tx n.
 Proof. unfold Origin. iauto. Qed.
 Hint Resolve origin_tx.
+
 Lemma origin_st : forall n t,
 Origin t n -> t <st msg n. 
 Proof. unfold Origin. iauto. Qed.
 Hint Resolve origin_st.
+
 Lemma origin_nopred_st : forall n t,
 Origin t n ->
 forall n', n' << n -> ~ t <st msg n'.
@@ -45,6 +837,8 @@ Proof.
   inversion ntheq as [msmsg].
   auto.
 Qed.
+Hint Resolve particular_min_smsg.
+
 Lemma particular_min_msg:
   forall {min actual_content},
     ((strand min) = [actual_content]) ->
@@ -55,6 +849,8 @@ Proof.
   erewrite particular_min_smsg.
   tauto. auto.
 Qed.
+Hint Resolve particular_min_msg.
+
 Lemma key_st_text_false : forall k t,
 (#k) <st (!t) -> False.
 Proof. intros. inversion H. Qed.
@@ -143,8 +939,7 @@ Proof.
   (* BOOKMARK *)
   forwards*: hd_pred_all.
   Admitted.
-
-
+Hint Resolve no_origin_after_rx.
 
 Lemma origin_imp_st_strand : forall t x s,
 Origin t x ->
@@ -193,3 +988,31 @@ Proof.
   inversion contra; eauto. 
 Qed.
 Hint Resolve no_encr_st.
+
+Lemma DolevYao_disjunction : forall s,
+DolevYao s ->
+((exists t, ~ set_In t PTexts /\ s = [ (+(!t)) ])
+ \/ 
+ (exists g, s = [(-g)])
+ \/ 
+ (exists g, s = [(-g) ; (+g) ; (+g)]) 
+ \/
+ (exists g h, s = [(-g) ; (-h) ; (+g*h)])
+ \/
+ (exists g h, s = [(-g*h) ; (+g) ; (+h)])
+ \/ 
+ (exists k, set_In k PKeys /\ s = [(+ (#k))])
+ \/ 
+ (exists h k, s = [(- (#k)) ; (-h) ; (+ {h}^[k])])
+ \/ 
+ (exists k' k h, Inv k' k /\ s = [(- (#k')) ; (- {h}^[k]) ; (+h)])).
+Proof.
+  intros. inversion H as [t tunk seq minstrand | 
+         g seq minstrand |
+         g seq minstrand |
+         g h seq minstrand |
+         g h seq minstrand |
+         k' kunk seq minstrand |
+         h k' seq minstrand |
+         h k' k'' inv seq minstrand]; iauto. 
+Qed.
