strandspace.v
@@ -18,7 +18,7 @@
  *)
 Require Import Logic List ListSet Arith Peano_dec Omega Ensembles.
 Require Import Finite_sets_facts Finite_sets Relation_Definitions.
-Require Import Relation_Operators Operators_Properties.
+Require Import Relation_Operators.
 Require Import CoLoRRelDec CoLoRRelSub.
 Require Import strictorder set_rep_equiv util.
 Require Import finite_set_builder.
@@ -59,13 +59,6 @@ Notation "{ m }^[ k ] " := (msg_encr k m) (at level 0, m at level 99, k at level
 
 Open Scope ss_scope.
 
-Definition eq_msg_dec : forall x y : Msg,  
-  {x = y} + {x <> y}.
-Proof.
-  decide equality.
-Qed.
-Hint Resolve eq_msg_dec.
-
 (* subterm relationship for messages *)
 (* subterm -> encompassing term -> Prop *)
 Inductive Subterm : Msg -> Msg -> Prop :=
@@ -93,25 +86,11 @@ Hint Constructors SMsg.
 Notation "(+ x )" := (msg_tx x) : ss_scope.
 Notation "(- x )" := (msg_rx x) : ss_scope.
 
-Definition eq_smsg_dec : forall x y : SMsg,  
-  {x = y} + {x <> y}.
-Proof.
- intros. decide equality.
-Qed. 
-Hint Resolve eq_smsg_dec.
-
 (* strand *)
 Definition Strand : Type := list SMsg.
 (* [REF 1] First sentence of Abstract: "sequence of events"  
    Haven't hit a better def, and they start using strands
    pretty early so I'm rolling with this. *)
-
-Definition eq_strand_dec : forall x y : Strand,  
-  {x = y} + {x <> y}.
-Proof.
- intros. decide equality.
-Qed.
-Hint Resolve eq_strand_dec.
 
 (* node in a strand space *)
 Definition Node : Type := {n: (Strand * nat) | (snd n) < (length (fst n))}.
@@ -207,105 +186,12 @@ Definition msg (n:Node) : Msg :=
    "Define uns_term(n) to be the unsigned part of the ith signed term 
     of the trace of s." *)
 
-Lemma node_smsg_msg_tx : forall n t,
-smsg(n) = (+ t) ->
-msg(n) = t.
-Proof.
-  intros n t nsmsg.
-  unfold msg. rewrite nsmsg. reflexivity. 
-Qed.
-
-Lemma node_smsg_msg_rx : forall n t,
-smsg(n) = (- t) ->
-msg(n) = t.
-Proof.
-  intros n t nsmsg.
-  unfold msg. rewrite nsmsg. reflexivity. 
-Qed.
-
 Definition is_tx (n:Node) : Prop :=
 exists t, smsg n = (+ t).
 
 Definition is_rx (n:Node) : Prop :=
 exists t, smsg n = (- t).
 
-Definition eq_node_dec : forall x y : Node,
- {x = y} + {x <> y}.
-Proof.
-  intros [[xs xn] xp] [[ys yn] yp].
-  destruct (eq_strand_dec xs ys) as [EQs | NEQs]; subst.
-  destruct (eq_nat_dec xn yn) as [EQn | NEQn]; subst.
-  left. rewrite (proof_irrelevance (lt yn (length ys)) xp yp). reflexivity.
-
-  right. intros C. inversion C. auto.
-  right. intros C. inversion C. auto.
-Qed.
-
-Lemma eq_nodes : forall x y : Node,
-index(x) = index(y) ->
-strand(x) = strand(y) ->
-x = y.
-Proof.
-  intros [[xs xn] xp] [[ys yn] yp] eq_index eq_strand.
-  simpl in eq_index. simpl in eq_strand. subst.
-  rewrite (proof_irrelevance (lt yn (length ys)) xp yp). reflexivity.
-Qed.
-
-Lemma nodes_eq : forall x y : Node,
-x = y ->
-index(x) = index(y) /\
-strand(x) = strand(y).
-Proof.
-  intros x y xyeq.
-  subst. auto.
-Qed.
-
-Lemma node_imp_strand_nonempty : forall s n,
-strand(n) = s ->
-length s > 0.
-Proof.
-  intros s n Hns.
-  destruct n. destruct x.
-  destruct n. simpl in l.
-  destruct s.
-  Case "s = []".
-    assert (s0 = nil). auto.
-  subst. inversion l.
-  Case "s = s :: s1".
-    simpl. omega.
-    simpl in l. 
-    assert (s0 = s). auto.
-    rewrite <- H.
-    omega.
-Qed.
-
-Lemma index_len_node : forall n,
-(index n) < length (strand n).
-Proof.
-  intros n.
-  destruct n. simpl. omega.
-Qed.
-
-Lemma node_indexing_equiv : forall n,
-nth_error (strand n) (index n) = Some (smsg n).
-Proof.
-  intros n.
-  unfold smsg. destruct node_smsg_valid. 
-  destruct n. simpl in *.
-  destruct x0.
-  rewrite e. simpl. reflexivity.
-Qed.
-
-Lemma strand_node : forall (s: Strand) (i: nat),
-i < length s ->
-exists n, strand n = s /\ index n = i.
-Proof.
-  intros s i len.  
-  eexists (exist _ (s,i) _). simpl.
-  split; reflexivity.
-Grab Existential Variables.
-  simpl. exact len.
-Qed.
 
 Inductive Comm : relation Node :=
 | comm :  forall n m t, ((smsg(n) = (+t) 
@@ -324,69 +210,6 @@ Hint Constructors Comm.
 
 Notation "a --> b" := (Comm a b) (at level 0, right associativity)  : ss_scope.
 
-Lemma comm_dec : forall x y,
-{x --> y} + {~ x --> y}.
-Proof.
-  intros x y.
-  remember (smsg x) as xsmsg. remember (smsg y) as ysmsg.
-  remember (strand x) as xstrand. remember (strand y) as ystrand.
-  destruct xsmsg.
-  Case "x (tx m)".
-    destruct ysmsg.
-    SCase "y (tx m0)".
-      right. intros contracomm. inversion contracomm; subst.
-      destruct H as [[xtx yrx] strandneq].
-      rewrite <- Heqysmsg in yrx. inversion yrx.      
-    SCase "y (rx m0)".
-      destruct (eq_msg_dec m m0) as [msgeq | msgneq].
-      SSCase "m = m0".
-        destruct (eq_strand_dec xstrand ystrand) as [strandeq | strandneq].
-        SSSCase "strands eq".
-          right. intros contracomm.
-          inversion contracomm; subst. destruct H as [msgs strandsneq].
-          apply strandsneq. exact strandeq. 
-        SSSCase "strands neq".
-          subst m0. left.
-          apply (comm x y m). split. split.
-          auto. auto. subst. exact strandneq.        
-      SSCase "m <> m0".
-        right. intros contracomm. inversion contracomm; subst. 
-        destruct H as [[xtx yrx] strandneq].
-        apply msgneq. rewrite <- Heqxsmsg in xtx.
-        rewrite <- Heqysmsg in yrx. inversion xtx; subst. 
-        inversion yrx; subst. reflexivity.
-  Case "x (rx m)".
-    right.
-    intros contracomm. inversion contracomm; subst.
-    destruct H as [[xtx yrx] strandneq].
-    rewrite <- Heqxsmsg in xtx. inversion xtx.
-Qed.
-
-Theorem comm_irreflexivity : forall n,
-~ n --> n.
-Proof.
-  intros n contraedge.
-  inversion contraedge; subst.
-  destruct H as [[txsmsg rxsmsg] strandneq].
-  apply strandneq. reflexivity.
-Qed.
-Hint Resolve comm_irreflexivity.
-
-Theorem comm_antisymmetry : 
-Antisymmetric Node Comm.
-Proof.
-  intros n m Hcomm contra.
-  assert False.
-  inversion Hcomm; subst.
-  inversion contra; subst.
-  destruct H as [H Hneq_s].
-  destruct H as [Htx1 Hrx1].
-  destruct H0 as [H Hneq_s2].
-  destruct H as [Htx2 Hrx2].
-  rewrite Htx2 in Hrx1. inversion Hrx1.
-  inversion H.
-Qed.
-Hint Resolve comm_antisymmetry.
 
 (* successor edge *)
 (* node's direct predecessor -> node -> Prop *)
@@ -400,50 +223,6 @@ Inductive Successor : relation Node :=
 
 Notation "a ==> b" := (Successor a b)  (at level 0, right associativity) : ss_scope. 
 
-Lemma succ_dec : forall x y,
-{x ==> y} + {~ x ==> y}.
-Proof.
-  intros x y.
-  remember (index x) as xi. remember (index y) as yi.
-  remember (strand x) as xstrand. remember (strand y) as ystrand.
-  destruct (eq_strand_dec xstrand ystrand) as [seq | sneq].
-  Case "strands eq".
-    destruct (eq_nat_dec yi (S xi)) as [succi | wrongi].
-    SCase "yi = S xi". left. apply (succ x y). rewrite <- Heqxstrand.
-      rewrite <- Heqystrand.  exact seq. omega.
-    SCase "yi <> S xi".
-      right. intros contrasucc. apply wrongi. inversion contrasucc; subst; omega.
-  Case "strands neq".
-    right. intros contrasucc. apply sneq. inversion contrasucc; subst; auto.
-Qed.  
-
-Theorem succ_irreflexivity : forall n,
-~n ==> n.
-Proof.
-  intros n edge.
-  inversion edge; subst. omega.
-Qed.
-Hint Resolve succ_irreflexivity.
-
-Theorem succ_antisymmetry :
-Antisymmetric Node Successor.
-Proof.
-  intros n m Hpe1 Hpe2.
-  destruct Hpe1. destruct Hpe2.
-  rewrite <- H0 in H2. omega.
-Qed.
-Hint Resolve succ_antisymmetry.
-
-Lemma single_succ : forall x y z,
-x ==> y ->
-x ==> z ->
-y = z.
-Proof.
-  intros x y z xy xz.
-  destruct xy.
-  destruct xz.
-  apply eq_nodes; auto; try omega; try congruence.
-Qed.
 
 (* succecessor multi edge (not nec. immediate succecessor) *)
 (* node's eventual succecessor -> node -> Prop *)
@@ -456,99 +235,6 @@ Hint Constructors clos_trans.
 
 Notation "a ==>+ b" := (StrandPath a b)  (at level 0, right associativity) : ss_scope.
 
-Lemma spath_imp_eq_strand : forall x y,
-x ==>+ y -> strand(x) = strand(y).
-Proof.
-  intros x y path.
-  induction path.
-  Case "step".
-    destruct H; auto.
-  Case "trans".
-    rewrite IHpath1.
-    rewrite IHpath2.
-    reflexivity.
-Qed.
-Hint Resolve spath_imp_eq_strand.
-
-Lemma spath_imp_index_lt : forall x y,
-x ==>+ y -> index(x) < index(y).
-Proof.
-  intros x y path.
-  induction path.
-  Case "step". inversion H; subst. omega.
-  Case "trans". omega.
-Qed.
-Hint Resolve spath_imp_index_lt.
-
-Lemma path_step_holds : forall x x' y,
-x ==>+ y ->
-x ==> x' ->
-x' = y \/ x' ==>+ y.
-Proof.
-  intros x x' y path. generalize dependent x'.
-  apply clos_trans_t1n in path.
-  induction path.
-    intros. left. eapply single_succ; eauto.
-    intros.
-    forwards*: (single_succ x y x'). subst.
-    right. apply clos_t1n_trans in path. auto.
-Qed.
-Hint Resolve path_step_holds.
-
-Lemma spath_from_props : forall x y,
-index(x) < index(y) ->
-(strand x) = (strand y) ->
-x ==>+ y.
-Proof.
-  intros x.
-  destruct x as [[xs xi] xp]. simpl in *. 
-  induction xi.
-    intros y ind streq.
-    destruct y as [[ys yi] yp]. simpl in *. 
-    induction yi. omega. 
-      destruct yi.
-        constructor. constructor. auto. simpl. reflexivity.
-        assert (snd (ys, S yi) < length (fst (ys, S yi))) as yp'. simpl. omega.
-        apply (t_trans Node Successor
-                 (exist (fun n : Strand * nat => snd n < length (fst n)) (xs, 0) xp)
-                 (exist (fun n : Strand * nat => snd n < length (fst n)) (ys, S yi) yp')
-                 (exist (fun n : Strand * nat => snd n < length (fst n)) (ys, S (S yi)) yp)).
-        apply IHyi. omega.
-        constructor. constructor. auto. simpl. omega.
-    intros y ind streq.
-    assert (snd (xs, xi) < length (fst (xs, xi))) as xp'. simpl. omega.
-    assert (exist (fun n : Strand * nat => snd n < length (fst n)) (xs, xi) xp') ==>
-         (exist (fun n : Strand * nat => snd n < length (fst n)) (xs, S xi) xp).
-      constructor. constructor. auto. simpl. omega.
-    assert (xi < index y). omega.
-    remember (IHxi xp' y H0 streq).
-    destruct (path_step_holds 
-              (exist (fun n : Strand * nat => snd n < length (fst n)) (xs, xi) xp')
-              (exist (fun n : Strand * nat => snd n < length (fst n)) (xs, S xi) xp)
-              y
-              s
-              H).
-    apply nodes_eq in H1. destruct H1. simpl in *.
-    constructor. constructor; auto. omega.
-    assumption.
-Qed.
-
-Lemma spath_irreflexivity : forall n,
-~ n ==>+ n.
-Proof.
-  intros n contra.
-  apply spath_imp_index_lt in contra.
-  omega.
-Qed.
-Hint Resolve spath_irreflexivity.
-
-Theorem spath_transitivity :
-Transitive Node StrandPath.
-Proof.
-  intros i j k Hij Hjk.
-  apply (t_trans Node Successor i j k Hij Hjk).
-Qed.
-Hint Resolve spath_transitivity.
 
 Definition SSEdge : relation Node :=
 union Comm Successor.
@@ -556,78 +242,12 @@ Hint Constructors or.
 
 Notation "a =-> b" := (SSEdge a b) (at level 30, right associativity) : ss_scope.
 
-Lemma ssedge_dec : forall x y,
-{x =-> y} + {~x =-> y}.
-Proof.
-  intros x y.
-  destruct (comm_dec x y) as [cxy | nocxy].
-  Case "Comm x y".
-    left. left. exact cxy.
-  Case "~Comm x y".
-    destruct (succ_dec x y) as [pxy | nopxy].
-    SCase "Successor x y".
-      left. right. exact pxy.
-    SCase "~Successor x y".
-      right. intros contrass.
-       destruct contrass.
-       SSCase "false Comm".
-         apply nocxy; exact H.
-       SSCase "false Successor".
-         apply nopxy; exact H.
-Qed.
-
-Theorem ssedge_irreflexivity : forall n,
-~ n =-> n.
-Proof.
-  intros n Hedge.
-  inversion Hedge; subst; auto.
-  eapply (comm_irreflexivity); eauto.
-  eapply (succ_irreflexivity); eauto.
-Qed.
-Hint Resolve ssedge_irreflexivity.
-
-Theorem ssedge_antisymmetry :
-Antisymmetric Node SSEdge.
-Proof.
-  intros n m Hss Hcontra.
-  inversion Hss; subst. inversion Hcontra; subst.
-  apply (comm_antisymmetry n m H) in H0. exact H0.
-  assert False.
-  inversion H; subst. inversion H0; subst.
-  inversion H1. apply H5. symmetry. exact H2.
-  inversion H1.
-  assert False.
-  inversion Hcontra; subst. inversion H; subst.
-  inversion H0; subst. inversion H3. apply H5.
-  symmetry. exact H1.
-  inversion H; subst. inversion H0; subst.
-  omega. inversion H0.
-Qed.
-Hint Resolve ssedge_antisymmetry.
 
 (* transitive closure of edges. *)
 Definition SSPath : relation Node := 
 clos_trans SSEdge.
 
 Notation "a << b" := (SSPath a b) (at level 0, right associativity) : ss_scope.
-
-Theorem spath_imp_sspath : forall i j,
-i ==>+ j -> i << j.
-Proof.
-  unfold SSPath.
-  intros i j Hpath.
-  induction Hpath.
-  constructor. right. exact H.
-  apply (t_trans Node SSEdge x y z IHHpath1 IHHpath2).
-Qed.  
-
-Theorem sspath_transitivity :
-Transitive Node SSPath.
-Proof.
-  unfold SSPath.
-  intros i j k Hij Hjk.
-  apply (t_trans Node SSEdge i j k Hij Hjk).
-Qed.
 
 (* transitive reflexive closure of edges. *)
 Definition SSPathEq : relation Node :=
@@ -636,33 +256,6 @@ Hint Constructors clos_refl_trans.
 
 Notation "a <<* b" := (SSPathEq a b) (at level 0, right associativity) : ss_scope.
 
-Theorem sspatheq_opts: forall n m,
-n <<* m -> n << m \/ n = m.
-Proof.
-  intros n m Hpatheq.
-  induction Hpatheq.
-  left. apply t_step. exact H.
-  right. reflexivity.
-  destruct IHHpatheq1 as [pathxy | eqxy].
-    destruct IHHpatheq2 as [pathyz | eqyz].
-      left. eapply t_trans. exact pathxy. exact pathyz.
-      subst y. left. exact pathxy.
-    destruct IHHpatheq2 as [pathyz | eqyz].
-      subst x. left. exact pathyz.
-      right. subst. reflexivity.
-Qed.
-
-Theorem sspatheq_transitivity :
-Transitive Node SSPathEq.
-Proof.
-  unfold Transitive.
-  intros i j k Hij Hjk.
-  destruct Hij. 
-    eapply rt_trans. eapply rt_step. exact H. 
-    exact Hjk. exact Hjk. 
-    eapply rt_trans. exact Hij1. eapply rt_trans.
-    exact Hij2. exact Hjk.
-Qed.
 
 (* In for members of pairs *)
 Inductive InPair {X:Type} (E:Ensemble (X*X)) (x:X): Prop :=
@@ -702,209 +295,18 @@ Record Bundle : Type := Bundle_def
 Definition StrandIn (s:Strand) (B:Bundle) :=
   forall n, (strand n) = s -> In Node (Nodes B) n.
 
-Lemma bundle_ssedge_inclusion : forall (B: Bundle) (n m: Node),
-n =-> m ->
-(In Node (Nodes B) n <-> In Node (Nodes B) m).
-Proof.
-  intros B n m ssedge. split; intros Hin.
-  destruct B as [N E finN finE valE uniqtx acyc]; simpl in *.
-  apply valE in ssedge. apply valE. constructor 2.
-  exists n. exact ssedge.
-  destruct B as [N E finN finE valE uniqtx acyc].
-  apply valE in ssedge. apply valE. constructor 1.
-  exists m. exact ssedge.
-Qed.
+
 
 Definition node_set_Ensemble_equiv (s: ListSet.set Node) (N:NodeSet) : Prop :=
 forall x, ListSet.set_In x s <-> In Node N x.
              
-Lemma sspath_imp_ssedge_l : forall x y,
-x << y ->
-exists x', x =-> x'.
-Proof.
-  intros x y sspath.
-  induction sspath.
-  exists y. exact H.
-  exact IHsspath1.
-Qed.  
-
-Lemma sspath_imp_ssedge_r : forall x y,
-x << y ->
-exists y', y' =->  y.
-Proof.
-  intros x y sspath.
-  induction sspath.
-  exists x. exact H.
-  exact IHsspath2.
-Qed.  
-
-Lemma restricted_to_set : forall (B:Bundle),
-exists s, is_restricted SSEdge s /\
-forall x, ListSet.set_In x s <-> In Node (Nodes B) x.
-Proof.
-  intros B.
-  destruct B as [N E finN finE valE uniqtx acyc]; simpl in *.
-  destruct valE as [EimpInN EimpSSEdge].
-  destruct (ensemble_imp_set Node eq_node_dec N finN) 
-    as [s [inAll [nodup [n [slen scard]]]]].
-  exists s.
-  split.
-  intros x y sspath.
-  split.
-  apply inAll. apply EimpInN. constructor. exists y. 
-  apply EimpSSEdge. exact sspath.
-  apply inAll. apply EimpInN. constructor 2. exists x. 
-  apply EimpSSEdge. exact sspath.
-  exact inAll.
-Qed.
-
-Lemma sspath_dec : forall (B: Bundle) (s: ListSet.set Node),
-node_set_Ensemble_equiv s (Nodes B) ->
-is_restricted SSEdge s ->
-forall x y, {x << y} + {~x << y}.
-Proof.
-  intros B s bset restrict.
-  destruct B as [N E finN finE valE uniqtx acyc]; simpl in *.
-  intros x y.
-  remember (restricted_dec_clos_trans_dec 
-              eq_node_dec 
-              ssedge_dec 
-              restrict) as alldec.
-  apply alldec.
-Qed.
-
-Lemma neq_sspatheq_imp_sspath : forall (x y: Node),
-x <> y ->
-x <<* y ->
-x << y.
-Proof.
-  intros x y neq patheqxy.
-  induction patheqxy.
-  Case "SSEdge x y".
-    apply t_step. exact H.
-  Case "x = y". assert False as F. apply neq. reflexivity. inversion F.
-  Case "x y z".
-    destruct (eq_node_dec y z) as [eqyz | neqyz].
-    SCase "y = z". subst y. apply IHpatheqxy1. exact neq.
-    SCase "y <> z". 
-      destruct (eq_node_dec x y) as [eqxy | neqxy].
-      SSCase "x = y". subst x. apply IHpatheqxy2. exact neqyz.
-      SSCase "x <> y". eapply t_trans. apply IHpatheqxy1. exact neqxy.
-        apply IHpatheqxy2. exact neqyz.
-Qed.      
-
-Lemma sspatheq_trans_cycle : forall (x y: Node),
-x <> y ->
-x <<* y ->
-y <<* x ->
-x << x.
-Proof.
-  intros x y neq patheqxy patheqyx.
-  eapply t_trans.
-  Case "path x y".
-    eapply neq_sspatheq_imp_sspath. exact neq. exact patheqxy.
-  Case "path y x".
-    eapply neq_sspatheq_imp_sspath. intros contra. subst.
-    apply neq. reflexivity.
-    exact patheqyx.
-Qed.
-
-(* Lemma 2.7a (partial order)  *)
-Lemma bunble_partial_order : forall (B:Bundle),
-Order Node SSPathEq.
-Proof.
-  intros B.
-  split.
-  Case "Reflexivity".
-    intros x. apply rt_refl. 
-  Case "Transitivity".
-    intros x y z xy yz.
-    eapply rt_trans. exact xy. exact yz.
-  Case "AntiSymmetry".
-    intros x y xy yz.
-    destruct B as [N E finN finE valE uniqtx acyc]; simpl in *.
-    destruct (eq_node_dec x y) as [xyeq | xyneq].
-    SCase "x = y". exact xyeq.
-    SCase "x <> y". 
-      assert (x << x) as contraxx.
-        eapply sspatheq_trans_cycle. exact xyneq.
-        exact xy. exact yz. apply acyc in contraxx. inversion contraxx.
-Qed.
-
-Lemma sspath_strict_order : forall (B: Bundle),
-StrictOrder Node SSPath.
-Proof.
-  intros B.
-  destruct B as [N E finN finE valE uniqtx acyc]; simpl in *.
-  split.
-  Case "Irreflexivity".
-    intros x. apply acyc.
-  Case "Transitivity".
-    apply sspath_transitivity.
-Qed.
 
 Definition set_minimal (N:NodeSet) (n:Node) : Prop :=
 In Node N n /\
 (forall x, In Node N x ->
            ~ x << n).
 
-(* Lemma 2.7b (non-empty subsets contain minimal members) *)
-Lemma bundle_subset_minimal : forall B N',
-Included Node N' (Nodes B) ->
-N' <> Empty_set Node ->
-exists min, set_minimal N' min.
-Proof.
-  intros B N' incl nempty.
-  remember B as bundle.
-  destruct bundle as [N E finN finE valE uniqtx acyc]; simpl in *.
-  assert (Finite Node N') as finN'. eapply Finite_downward_closed.
-    exact finN. exact incl.
-  destruct (finite_cardinal Node N' finN') as [n card].
-  destruct n. inversion card. rewrite H in nempty.
-  assert False as F. apply nempty. reflexivity. inversion F.
-  destruct (restricted_to_set B) as [s [restricted setequiv]].
-  assert (forall x y, {x << y} + {~ x << y}) as rdec.
-  apply (sspath_dec B s). exact setequiv. exact restricted.  
-  destruct (minimal_finite_ensemble_mem 
-              Node 
-              eq_node_dec 
-              SSPath 
-              rdec
-              (sspath_strict_order B) 
-              N' 
-              n 
-              card) as [min [minIn nolt]].
-  exists min. split. exact minIn. exact nolt.
-Qed.
 
-(* Lemma 2.8 - set minimal is tx *)
-Lemma minimal_is_tx : forall B N',
-Included Node N' (Nodes B) ->
-(forall m m' : Node, (In Node (Nodes B) m 
-               /\ In Node (Nodes B) m'
-               /\ msg(m) = msg(m')) -> (* ADDED in N conditions *)
-               (In Node N' m <-> In Node N' m')) ->
-forall n, set_minimal N' n ->
-is_tx n.
-Proof.
-  intros B N' sub incl n setmin.
-  remember B as bundle.
-  destruct bundle as [N E finN finE valE uniqtx acyc]; simpl in *.
-  assert ((Nodes B) = N) as NB. subst B. simpl. reflexivity.
-  remember (smsg n) as nsmsg. symmetry in Heqnsmsg.
-  destruct nsmsg.
-  exists m. exact Heqnsmsg.
-  unfold ExistsUniqueTx in uniqtx.
-  assert (In Node N n) as nIn. destruct setmin; auto.
-  destruct (uniqtx n m nIn Heqnsmsg) as [[ntx [ntxsmsg [commn inE]]] uniq].
-  assert False as F. destruct setmin. apply (H0 ntx). eapply incl.
-    split. rewrite <- NB. eapply bundle_ssedge_inclusion. 
-    constructor. exact commn. rewrite NB. exact nIn. 
-    split. exact nIn. apply node_smsg_msg_tx in ntxsmsg. 
-    apply node_smsg_msg_rx in Heqnsmsg. rewrite Heqnsmsg. exact ntxsmsg. 
-    exact H. constructor. constructor. exact commn.
-  inversion F.
-Qed.
 
 Definition OccursIn (t:Msg) (n:Node) : Prop :=
  t <st msg(n).
@@ -933,21 +335,6 @@ is_tx n
 /\ t <st msg(n)
 /\ forall n', n' << n -> ~t <st msg(n').
 
-Lemma Origin_imp_strict_defs : forall I t n,
-(forall t', t <st t' <-> In Msg I t') ->
-Origin t n ->
-Origin_with_Ex_Set t n.
-Proof.
-  intros I t n Iprop Orig.
-  exists I. split. exact Iprop.
-  destruct Orig as [ntx [nsub nosucc]].
-  split. exists (msg n).
-  split. apply Iprop in nsub. exact nsub.
-  destruct ntx. erewrite node_smsg_msg_tx. exact H. exact H.
-  intros n' succ contraIn.
-  apply nosucc in succ. apply Iprop in contraIn. contradiction.
-Qed.
-
 Definition UniqOrigin (t:Msg) : Prop :=
 exists n, Origin t n
 /\ forall m, Origin t m -> n = m.
@@ -955,55 +342,6 @@ exists n, Origin t n
    "An unsigned term t is uniquely originating iff t originates on
     a unique n." *)
 
-(* Lemma 2.9 originating occurrence at minimal element *)
-Lemma min_origin : forall B N' n t,
-(forall m, (In Node (Nodes B) m 
-           /\ Subterm t (msg(m))) -> 
-           In Node N' m) ->
-(forall m, In Node N' m -> 
-           (In Node (Nodes B) m 
-           /\ Subterm t (msg(m)))) ->
-set_minimal N' n ->
-Origin t n.
-Proof.
-  intros B N' n t N'deff N'defb nmin.
-  remember B as bundle.
-  destruct bundle as [N E finN finE valE uniqtx acyc]; simpl in *.
-  assert (N = Nodes B) as NB. subst B. simpl; reflexivity.
-  assert (In Node N' n) as nIn. destruct nmin; auto.
-  assert (t <st (msg n)) as tsubn.
-    apply (N'defb n) in nIn. destruct nIn; auto.
-  assert (is_tx n) as nistx.
-    assert (Included Node N' N) as incl.
-      intros x xIn. apply N'defb in xIn. destruct xIn; auto.
-    rewrite NB in incl. apply (minimal_is_tx B N' incl).
-    intros x y eqmsg.
-    destruct eqmsg as [xIn [yIn eqmsg]].
-    split; intros Hin.
-    Case "m in -> m' in".
-      apply N'defb in Hin. destruct Hin as [xInN tsubx]. 
-      assert (Subterm t (msg y)) as ysubt. rewrite <- eqmsg.
-        exact tsubx.
-      apply N'deff. split. rewrite NB. exact yIn. exact ysubt.
-    Case "m' in -> m in".
-      apply N'defb in Hin. destruct Hin as [yInN tsuby].
-      apply N'deff. split. rewrite NB. exact xIn. 
-      assert (Subterm t (msg x)) as xsubt. rewrite eqmsg.
-        exact tsuby.
-      exact xsubt. 
-    exact nmin.
-  split. exact nistx.
-  split. exact tsubn.
-  intros n' succn' contrasub.
-  assert (In Node N' n') as n'In.
-    apply N'deff. split.
-    destruct valE as [pairImpN HInEedge].
-    apply pairImpN. left.
-    destruct (sspath_imp_ssedge_l n' n succn') as [x n'edge].
-    exists x. apply HInEedge. exact n'edge. exact contrasub.
-  destruct nmin as [nIn2 noprev]. apply (noprev n'). exact n'In.
-  exact succn'.
-Qed.
 
 (* Axiom 1 -- provable in this context *)
 Theorem free_encryption : forall m1 m2 k1 k2,
@@ -1048,76 +386,6 @@ match m with
 end.
 (* [REF 1] Definition 2.10 *)
 
-
-(* Proposition 2.12 *)
-Lemma encr_subterm_imp : forall k k' h h',
-k <> k' ->
-{h'}^[k'] <st {h}^[k] ->
-{h'}^[k'] <st h.
-Proof.
-  intros k k' h h' kneq st.
-  inversion st; subst.
-  assert False. apply kneq. reflexivity. contradiction.
-  exact H1.
-Qed.
-
-Lemma st_dec : forall a b,
-{a <st b} + {~ a <st b}.
-Proof.
-  intros a b.
-  induction b.
-  Case "b = txt".
-    destruct a.
-    SCase "a = txt".
-      destruct (eq_text_dec t t0).
-        subst t. left. auto.
-        right. intros contra. inversion contra. 
-        symmetry in H1. contradiction.
-    SCase "a = key". right. intros contra. inversion contra.
-    SCase "a = join". right. intros contra. inversion contra.
-    SCase "a = encr". right. intros contra. inversion contra.
-  Case "b = key".
-    destruct a.
-    SCase "a = txt". right. intros contra. inversion contra.
-    SCase "a = key".
-      destruct (eq_key_dec k k0).
-        subst k. left. auto.
-        right. intros contra. inversion contra. 
-        symmetry in H1. contradiction.
-    SCase "a = join". right. intros contra. inversion contra.
-    SCase "a = encr". right. intros contra. inversion contra.
-  Case "b = join".
-    destruct IHb1.
-    SCase "a <st b1". left. apply st_join_l. exact s.
-    SCase "~a <st b1". 
-      destruct IHb2.
-      SSCase "a <st b2". left. apply st_join_r. exact s.
-      SSCase "~a <st b2". 
-        destruct (eq_msg_dec a (b1 * b2)).
-        SSSCase "a = b1 * b2".
-          subst a. left. constructor.
-        SSSCase "a <> b1 * b2".
-          right. intros contra. inversion contra; subst; try(contradiction).
-          apply n1. reflexivity.
-  Case "b = encr".
-    destruct IHb.
-      left. apply st_encr. exact s.
-      destruct (eq_msg_dec a ({b}^[k])). subst.
-      left. constructor.
-      right. intros contra. inversion contra. subst.
-      apply n0. reflexivity.
-      contradiction.
-Qed.
-
-Fixpoint st_on_strand (t:Msg) (s:Strand) : bool :=
-match s with
-| nil => false
-| x :: xs => 
-  if st_dec t (smsg_msg x)
-  then true
-  else st_on_strand t xs
-end.
-
 (* Meta Strand Space properties/objects *)
 (* [REF 1] 
            Page 4 "One may think of a strand space as containing all the 
@@ -1137,12 +405,6 @@ Definition PenetratorNode (n:Node) := ~RegularNode n.
 Variable PenetratorModel : Strand -> Prop.
  Hypothesis penetrator_behaviour : 
    forall s, PenetratorStrand s -> PenetratorModel s.
-
-Theorem align_dec : forall s,
-{RegularStrand s} + {PenetratorStrand s}.
-Proof.
-  intros s. destruct (set_In_dec eq_strand_dec s Protocol); auto.
-Qed.
 
 (* Keys known to penetrators *)
 Variable PKeys : set Key.
